# Limits and Derivatives (cont.)

### Example 6

Heaviside function:

`H(t) = { 0 : t < 0; 1 : t >= 0 }`

`lim[t->0](H(t)) = DNE`

## One-sided limits

Limit coming from the left or the right (negative or positive).

Limit of `f(x)` as `x` approaches `a` from the left (`x < a`):

`lim-[x->a](f(x)) = L`

Limit of `f(x)` as `x` approaches `a` from the right (`x < a`):

`lim+[x->a](f(x)) = L`

Note the negative and positive signs to denote from which side `x` is approaching `a`.

`lim[x->a](f(x)) = L` if and only if `lim-[x->a](f(x)) = L` and `lim+[x->a](f(x)) = L`.

### Example 7

The graph of a function `g` is given. Use it to state the values (if they exist) of the following:

- `lim-[x->2](g(x)) = 3`
- `lim+[x->2](g(x)) = 1`
- `lim[x->2](g(x)) = DNE`
- `lim-[x->5](g(x)) = 2`
- `lim+[x->5](g(x)) = 2`
- `lim[x->5](g(x)) = 2`

### Example 8

Find `lim[x->0](1 / x^2)` if it exists.

`lim[x->0](1 / x^2) = inf`

## Infinite limits

**Remark**: infinity is only a symbol, not a number.

Infinity can be negative or positive.

`x = a` is a vertical asymptote of `y = f(x)` if one of the following is true:

- `lim[x->a](f(x)) = inf`
- `lim-[x->a](f(x)) = inf`
- `lim+[x->a](f(x)) = inf`
- `lim[x->a](f(x)) = -inf`
- `lim-[x->a](f(x)) = -inf`
- `lim+[x->a](f(x)) = -inf`

### Example 9

Find `lim+[x->3](2x / (x - 3))` and `lim-[x->3](2x / (x - 3))`

`lim+[x->3](2x / (x - 3)) = inf`

`lim-[x->3](2x / (x - 3)) = -inf`

# Calculating Limits Using the Limit Laws

(finally).

## Limit Laws

Suppose that `c` is a constant, and that `lim[x->a](f(x))` and `lim[x->a](g(x))` both exist.

The limit laws may also be applied to one-sided limits.

- `lim[x->a](f(x) + g(x)) = lim[x->a](f(x)) + lim[x->a](g(x))`

- `lim[x->a](f(x) - g(x)) = lim[x->a](f(x)) - lim[x->a](g(x))`

- `lim[x->a](c * f(x)) = c * lim[x->a](f(x))`

- `lim[x->a](f(x) * g(x)) = lim[x->a](f(x)) * lim[x->a](g(x))`

- `lim[x->a](f(x) / g(x)) = lim[x->a](f(x)) / lim[x->a](g(x))` if `lim[x->a](g(x)) != 0`

- `lim[x->a](f(x)^n) = (lim[x->a](f(x)))^2` where `n` is a positive integer.

- `lim[x->a](c) = c`

- `lim[x->a](x^n) = a^n` where `n` is a positive integer.

- `lim[x->a](root(n, x)) = root(n, a)` where `n` is a positive integer.
    - If `n` is even, we assume `a > 0`.

- `lim[x->a](root(n, f(x))) = root(n, lim[x->a](f(x)))` where `n` is a positive integer.
    - If `n` is even, we assume `lim[x->a](f(x)) > 0`.

### Example 2

Evaluate the following limits and justify each step.

```
lim[x->5](2x^2 - 3x + 4)

    = lim[x->5](2x^2) - lim[x->5](3x) + lim[x->5](4)

    = 2 * lim[x->5](x^2) - 3 * lim[x->5](x) + 4

    = 2 * 5^2 - 3 * 5 + 4

    = 39
```

```
lim[x->(-2)]((x^3 + 2x^2 - 1) / (5 - 3x))

    = lim[x->(-2)](x^3 + 2x - 1) / lim[x->(-2)](5 - 3x)

    = lim[x->(-2)](x^3) + 2 * lim[x->(-2)](x) - lim[x->(-2)](1) / lim[x->(-2)](5) - 3 * lim[x->(-2)](x)

    = ((-2)^3 + 2 * (-2) - 1) / (5 - 3 * -2)

    = -(1 / 11)
```

## Direct Substitution Property

If `f` is a polynomial or rational function, and `a` is in the domain of `f`:

`lim[x->a](f(x)) = f(a)`

### Example

Find `lim[x->2]((x^2 - 1) / (x - 1))`

Since `(x^2 - 1) / (x - 1)` is a rational function we can use the direct substitution property.

```
lim[x->2]((x^2 - 1) / (x - 1))

    = (2^2 - 1) / (2 - 1)

    = 3
```

### Example 3

```
lim[x->1](x^2 - 1 / x - 1)

    = lim[x->1]((x + 1)(x - 1) / (x - 1))

    = lim[x->1](x + 1)

    = 2
```

### Example 4

Find `lim[x->1](g(x))` where `g(x) = { x + 1 : x != 1; pi : x == 1}`

`lim[x->1](g(x)) = 2`

When dealing with limits we do not care about the value of `g(x)` at `a`, rather we care about what
value `g(x)` **approaches** as `x` approaches `a`.

Therefore for a function such as `g(x)`, we can ignore the case where `x == 1` and define the limit
as `x + 1`.

### Example 5

```
lim[h->0](((3 + h)^2 - 9) / h)

    = lim[h->0]((9 + 6h + h^2 - 9) / h)

    = lim[h->0]((6h + h^2) / h)

    = lim[h->0]((6 + h) / 1)

    = 6
```

### Example 6

```
lim[t->0]((sqrt(t^2 + 9) - 3) / t^2)

    = lim[t->0](((sqrt(t^2 + 9) - 3) / t^2) * ((sqrt(t^2 + 9) + 3) / sqrt(t^2 + 9) + 3))

    = lim[t->0]((t^2 + 9 - 9) / t^2 * (sqrt(t^2 + 9) + 3))





